Risc0/Gadgets/ComputeDecode/Proofs.lean
@@ -17,48 +17,39 @@ theorem constraints_of_witness
   {x₀ x₁ x₂ x₃ : Felt}
   {output : BufferAtTime}
   (h : output.length = 18) 
-  (h₁ : output.all Option.isSome) 
+  -- (h₁ : output.all Option.isSome) 
   (h_isBytes: ∀ (i : ℕ), i < (4 : ℕ) → isByte (Option.get! (List.get! [some x₀, some x₁, some x₂, some x₃] i))):
   (Witness.Code.run (Witness.start_state [x₀, x₁, x₂, x₃])) output →
     (Constraints.Code.run (Constraints.start_state [x₀, x₁, x₂, x₃] output)) := by
-  rcases output with _ | ⟨y0, output⟩ <;> simp at *
-  rcases output with _ | ⟨y1, output⟩ <;> simp at *
-  rcases output with _ | ⟨y2, output⟩ <;> simp at *
-  rcases output with _ | ⟨y3, output⟩ <;> simp at *
-  rcases output with _ | ⟨y4, output⟩ <;> simp at *
-  rcases output with _ | ⟨y5, output⟩ <;> simp at *
-  rcases output with _ | ⟨y6, output⟩ <;> simp at *
-  rcases output with _ | ⟨y7, output⟩ <;> simp at *
-  rcases output with _ | ⟨y8, output⟩ <;> simp at *
-  rcases output with _ | ⟨y9, output⟩ <;> simp at *
-  rcases output with _ | ⟨y10, output⟩ <;> simp at *
-  rcases output with _ | ⟨y11, output⟩ <;> simp at *
-  rcases output with _ | ⟨y12, output⟩ <;> simp at *
-  rcases output with _ | ⟨y13, output⟩ <;> simp at *
-  rcases output with _ | ⟨y14, output⟩ <;> simp at *
-  rcases output with _ | ⟨y15, output⟩ <;> simp at *
-  rcases output with _ | ⟨y16, output⟩ <;> simp at *
-  rcases output with _ | ⟨y17, output⟩ <;> simp at *
-  rcases output with _ | ⟨_, output⟩ <;> simp at *
-  rw [Witness.WP.closed_form, decoder_closed_form_equiv_decoder_direct_spec]
-  unfold decoder_direct_spec
-  simp [Instruction.fromWords]
-  intro h0 h1 h2 h3 h4 h5 h6 h7 h8 h9 h10 h11 h12 h13 h14 h15 h16 h17
-  subst h0 h1 h2 h3 h4 h5 h6 h7 h8 h9 h10 h11 h12 h13 h14 h15 h16 h17
-  rw [Constraints.WP.closed_form]
-  have h_toWords := @toWords_fromWords [x₀, x₁, x₂, x₃] (by simp) h_isBytes (by {
-    intros i h_i
-    rcases i with _ | i <;> simp at *
-    rcases i with _ | i <;> simp at *
-    rcases i with _ | i <;> simp at *
-    rcases i with _ | i <;> simp at *
-    tauto
-  })
-  unfold Instruction.toWords Instruction.fromWords at h_toWords
-  simp at h_toWords
-  rcases h_toWords with ⟨h_toWords₀, h_toWords₁, h_toWords₂, h_toWords₃⟩
-  rw [←h_toWords₀, ←h_toWords₁, ←h_toWords₂, ←h_toWords₃] 
-  aesop
+    rcases output with _ |
+      ⟨y0, _ | ⟨y1, _ | ⟨y2, _ | ⟨y3, _ | ⟨y4, _ | ⟨y5, _ | ⟨y6, _ | ⟨y7, _ | ⟨y8, _ | ⟨y9, _ |
+      ⟨y10, _ | ⟨y11, _ | ⟨y12, _ | ⟨y13, _ | ⟨y14, _ | ⟨y15, _ | ⟨y16, _ | ⟨y17, ⟨_ | _⟩⟩⟩⟩⟩⟩⟩⟩⟩⟩⟩⟩⟩⟩⟩⟩⟩⟩⟩ <;>
+      simp at h
+    rw [Witness.WP.closed_form, decoder_closed_form_equiv_decoder_direct_spec, decoder_direct_spec]
+    rintro ⟨⟨⟨_⟩, h₃⟩, h₄⟩
+    simp only [List.map, List.cons.injEq, and_true] at h₃ 
+    
+
+
+    -- simp? [Instruction.fromWords]
+    -- intro h0 h1 h2 h3 h4 h5 h6 h7 h8 h9 h10 h11 h12 h13 h14 h15 h16 h17
+    -- subst h0 h1 h2 h3 h4 h5 h6 h7 h8 h9 h10 h11 h12 h13 h14 h15 h16 h17
+    -- rw [Constraints.WP.closed_form]
+    -- have h_toWords := @toWords_fromWords [x₀, x₁, x₂, x₃] (by simp) h_isBytes (by {
+    --   intros i h_i
+    --   rcases i with _ | i <;> simp at *
+    --   rcases i with _ | i <;> simp at *
+    --   rcases i with _ | i <;> simp at *
+    --   rcases i with _ | i <;> simp at *
+    --   tauto
+    -- })
+    -- unfold Instruction.toWords Instruction.fromWords at h_toWords
+    -- simp at h_toWords
+    -- rcases h_toWords with ⟨h_toWords₀, h_toWords₁, h_toWords₂, h_toWords₃⟩
+    -- rw [←h_toWords₀, ←h_toWords₁, ←h_toWords₂, ←h_toWords₃] 
+    -- aesop
+
+#exit
 
 theorem spec_of_constraints {x₀ x₁ x₂ x₃ : Felt}
   {y0 y1 y2 y3 y4 y5 y6 y7 y8 y9 y10 y11 y12 y13 y14 y15 y16 y17 : Felt} :
